\paragraph{Example}
Suppose following initial conditions: $\eta(0) = L$ and $\dot{\eta} = 0$
Then $A=L$ and $\varphi = 0$.
\subsection{$N$ non-coupled oscillators}
$$L  = \sum_i \left( \frac{1}{2}m_i\dot{\eta}_i^2  - \frac{1}{2} k_i  \eta_i^2\right)$$
Movement equations are:
$$\ddot{\eta}_i = -\frac{k_i}{m_i} \eta_i$$
$$\eta_i = a e^{i\omega_i t}$$
Define 
$$T = (T)_{ij}$$
In our case
$T_{ij} = \delta_{ij} m_i$
And define $$\eta = \begin{pmatrix}\eta_1 \\ \vdots \\ \eta_n\end{pmatrix}$$
And $V_{ij} = \delta_{ij} k_i$.

Then
$$T\dot{\eta} = \begin{pmatrix} \sum T_{1i}\eta_i \\ \vdots \\ \sum T_{Ni}\eta_i \end{pmatrix}$$ 
$$\dot{\eta}^T T\dot{\eta} = \sum_{i,j} T_{ij} \dot{\eta}_i \dot{\eta}_j$$
For our case $$\dot{\eta}^T T\dot{\eta} = \sum_{i,j} \delta_{ij} m_i \dot{\eta}_i \dot{\eta}_j = \sum_i m_i \dot{\eta}_i^2$$
and
$$\eta^T V \eta = \sum_i k_i \eta^2_i$$
$$L = \frac{1}{2} \dot{\eta}^T T\dot{\eta} + \frac{1}{2} \eta^T V \eta $$


\subsection{$N$ coupled oscillators}
Since potentials are now dependent of each other, lets write Taylor series:
$$V(\eta_1, \dots, \eta_N) = \underbrace{V_0}_{0} + \underbrace{\frac{\partial V}{\partial \eta_i}_{\eta=0} \eta_i}_{0} + \frac{1}{2}\frac{\partial^2 V}{\partial \eta_i \partial \eta_j}_{\eta=0} \eta_i \eta_j + \dots$$
Thus
$$V = \frac{1}{2} \frac{\partial^2 V}{\partial \eta_i \partial \eta_j}_{\eta=0} \eta_i \eta_j = \frac{1}{2} \eta^T V \eta$$
The potential matrix is
$$V_{ij} = \frac{\partial^2 V}{\partial \eta_i \partial \eta_j}$$

Now, for kinetic energy:
$$T = \sum_{i} \frac{1}{2} m_j \dot{\eta}^2_i$$
Then $T_{ij} = \delta_{ij} m_i$.

For generalized coordinates:
$$\dot{x}_i = \sum_j \frac{\partial x_i}{\partial q_j} \dot{q}_j$$
So
$$T = \frac{1}{2} \sum_i m_i \left( \sum_j \frac{\partial x_i}{\partial q_j} \dot{q}_j \right)^2 = \frac{1}{2} \sum_i m_i \sum_j \frac{\partial x_i}{\partial q_j} \dot{q}_j \sum_k \frac{\partial x_i}{\partial q_k} \dot{q}_k = \frac{1}{2} \sum_{j,k} \left( \underbrace{\sum_i m_i   \frac{\partial x_i}{\partial q_j} \frac{\partial x_i}{\partial q_k}}_{m_{jk}(q)}\right) \dot{q}_j \dot{q}_k $$

Since we all elements in $T$ are at least second-order , we can approximate $m_{jk}(q) = m_{jk}(0)$ since everything else is negligible:
$$T_{ij} = \frac{1}{2} \sum_{i,j} m_{jk_0} \dot{\eta}_j \dot{\eta}_k$$
i.e. $T_{jk} = m_{jk_0}$